working + linked very simple demo.

tests/demo/A_o.v
@@ -8,43 +8,38 @@ From Demo Require
      A_cpp A_cpp_spec A_cpp_proof.
 Import A_hpp_spec.
 
-Definition module_link (a b : list Decl) : list Decl := a ++ b.
-
-Axiom denoteModule_link : forall nss a b,
-    denoteModule nss (module_link a b) -|- denoteModule nss a ** denoteModule nss b.
-
 (* todo(gmm): I'm a bit confused about the appropriate specification of linking
  *)
-Lemma wand_apply : forall A B : mpred,
-    A |-- (A -* B) ** B.
+Lemma wand_apply : forall A B F F' : mpred,
+    F |-- A ** F' ->
+    (A -* B) ** F |-- B ** F'.
 Proof.
   intros.
-Abort.
-
-Lemma lob_link : forall A B : mpred,
-    ((|> A) -* B) ** ((|> B) -* A) |-- A ** B.
-Proof.
-  intros.
-  eapply sepSPAdj'.
-  rewrite <- empSPL.
+  rewrite H.
+  work.
+  rewrite sepSPC.
   eapply sepSPAdj.
-  rewrite <- (landtrueR empSP).
-  apply landL2.
-  eapply spec_lob.
-Abort.
-    (* |>A ==> B
-     * |>B ==> A
-     * A //\\ B
-     *)
+  reflexivity.
+Qed.
+
+Require Import Cpp.Linking.
 
 Theorem A_o_sound (resolve : _)
-: denoteModule nil (module_link A_hpp.module A_cpp.module)
-  |-- cglob' (resolve:=resolve) A__foo A__foo_spec **
+: |-- denoteModule nil (module_link A_hpp.module A_cpp.module) -*
+      cglob' (resolve:=resolve) A__foo A__foo_spec **
       cglob' (resolve:=resolve) A__bar A__bar_spec.
 Proof.
+  eapply spec_lob.
+  eapply wandSPAdj.
+  rewrite denote_module_dup at 2.
   rewrite denoteModule_link.
-  rewrite (A_cpp_proof.A_cpp_sound resolve).
-  rewrite (A_hpp_proof.A_hpp_sound resolve).
-  unfold A_hpp_spec.
-  unfold A_cpp_spec.A_cpp_spec.
-Abort. (* todo(gmm): finish this proof *)
+  rewrite (A_cpp_proof.A_cpp_sound resolve) at 2.
+  rewrite (A_hpp_proof.A_hpp_sound resolve) at 2.
+  unfold A_hpp_spec, A_cpp_spec.A_cpp_spec.
+  do 2 Discharge.perm_right ltac:(idtac; Discharge.perm_left ltac:(eapply wand_apply)).
+  rewrite illater_wandSP.
+  rewrite <- illater_sepSP.
+  Discharge.perm_right ltac:(idtac; Discharge.perm_left ltac:(eapply wand_apply)).
+  rewrite <- spec_later_weaken.
+  Discharge.discharge ltac:(Discharge.canceler fail eauto) eauto.
+Qed.
